Started moving towards chained environments

11FlatMemory/FlatMemory.thy
@@ -1,58 +1,64 @@
 theory FlatMemory
-  imports "../09HeapMemory/HeapMemory"
+  imports "../10ChainedEnvironment/ChainedEnvironment"
 begin
 
 datatype flat_state = 
-  FS "nat heap" "ptr list" "nat list list" (code: "byte_code list")
+  FS "nat heap" "ptr heap" "ptr list" "nat list" (code: "byte_code list")
 
-fun get_closure :: "nat heap \<Rightarrow> nat \<Rightarrow> hclosure" where
+fun get_closure :: "nat heap \<Rightarrow> nat \<Rightarrow> ceclosure" where
   "get_closure h p = (case hlookup h p of
-      0 \<Rightarrow> HConst (hlookup h (Suc p))
-    | Suc x \<Rightarrow> HLam (hlookup_list h (Suc (Suc p)) x) (hlookup h (Suc p)))"
+      0 \<Rightarrow> CEConst (hlookup h (Suc p))
+    | Suc x \<Rightarrow> CELam (hlookup h (Suc p)) (hlookup h (Suc (Suc p))))"
+
+fun flat_lookup :: "ptr heap \<Rightarrow> ptr \<Rightarrow> nat \<rightharpoonup> ptr" where
+  "flat_lookup h 0 x = None"
+| "flat_lookup h (Suc 0) x = None"
+| "flat_lookup h (Suc (Suc p)) 0 = Some (hlookup h p)"
+| "flat_lookup h (Suc (Suc p)) (Suc x) = flat_lookup h (hlookup h (Suc p)) x"
 
 inductive evalf :: "flat_state \<Rightarrow> flat_state \<Rightarrow> bool" (infix "\<leadsto>\<^sub>f" 50) where
-  evf_lookup [simp]: "cd ! pc = BLookup x \<Longrightarrow> lookup env x = Some v \<Longrightarrow> 
-    FS h vs ((Suc pc # env) # sfs) cd \<leadsto>\<^sub>f FS h (v # vs) ((pc # env) # sfs) cd"
-| evf_pushcon [simp]: "cd ! pc = BPushCon k \<Longrightarrow> halloc_list h [0, k] = (h', v) \<Longrightarrow>
-    FS h vs ((Suc pc # env) # sfs) cd \<leadsto>\<^sub>f FS h' (v # vs) ((pc # env) # sfs) cd"
-| evf_pushlam [simp]: "cd ! pc = BPushLam pc' \<Longrightarrow> 
-    halloc_list h (Suc (length env) # pc' # env) = (h', v) \<Longrightarrow>
-      FS h vs ((Suc pc # env) # sfs) cd \<leadsto>\<^sub>f FS h' (v # vs) ((pc # env) # sfs) cd"
-| evf_apply [simp]: "cd ! pc = BApply \<Longrightarrow> get_closure h v2 = HLam env' pc' \<Longrightarrow>
-    FS h (v1 # v2 # vs) ((Suc pc # env) # sfs) cd \<leadsto>\<^sub>f
-      FS h vs ((pc' # v1 # env') # (pc # env) # sfs) cd"
-| evf_return [simp]: "cd ! pc = BReturn \<Longrightarrow> 
-    FS h vs ((Suc pc # env) # sfs) cd \<leadsto>\<^sub>f FS h vs sfs cd"
-| evf_jump [simp]: "cd ! pc = BJump \<Longrightarrow> get_closure h v2 = HLam env' pc' \<Longrightarrow>
-    FS h (v1 # v2 # vs) ((Suc pc # env) # sfs) cd \<leadsto>\<^sub>f FS h vs ((pc' # v1 # env') # sfs) cd"
+  evf_lookup [simp]: "cd ! pc = BLookup x \<Longrightarrow> flat_lookup env p x = Some v \<Longrightarrow> 
+    FS h env vs (Suc pc # p # sfs) cd \<leadsto>\<^sub>f FS h env (v # vs) (pc # p # sfs) cd"
+| evf_pushcon [simp]: "cd ! pc = BPushCon k \<Longrightarrow> halloc h 0 = (h1, v) \<Longrightarrow> halloc h1 k = (h2, v') \<Longrightarrow> 
+    halloc h2 0 = (h3, v2) \<Longrightarrow>
+      FS h env vs (Suc pc # p # sfs) cd \<leadsto>\<^sub>f FS h3 env (v # vs) (pc # p # sfs) cd"
+| evf_pushlam [simp]: "cd ! pc = BPushLam pc' \<Longrightarrow> halloc h 1 = (h1, v) \<Longrightarrow> 
+    halloc h1 p = (h2, v') \<Longrightarrow> halloc h2 pc' = (h3, v2) \<Longrightarrow>
+      FS h env vs (Suc pc # p # sfs) cd \<leadsto>\<^sub>f FS h3 env (v # vs) (pc # p # sfs) cd"
+| evf_apply [simp]: "cd ! pc = BApply \<Longrightarrow> get_closure h v2 = CELam p' pc' \<Longrightarrow>
+    halloc env v1 = (env1, p1) \<Longrightarrow> halloc env1 p' = (env2, p2) \<Longrightarrow> 
+      FS h env (v1 # v2 # vs) (Suc pc # p # sfs) cd \<leadsto>\<^sub>f 
+        FS h env2 vs (pc' # Suc p2 # pc # p # sfs) cd"
+| evf_return [simp]: "cd ! pc = BReturn \<Longrightarrow> FS h env vs (Suc pc # p # sfs) cd \<leadsto>\<^sub>f FS h env vs sfs cd"
+| evf_jump [simp]: "cd ! pc = BJump \<Longrightarrow> get_closure h v2 = CELam p' pc' \<Longrightarrow>
+    halloc env v1 = (env1, p1) \<Longrightarrow> halloc env1 p' = (env2, p2) \<Longrightarrow> 
+      FS h env (v1 # v2 # vs) (Suc pc # p # sfs) cd \<leadsto>\<^sub>f FS h env2 vs (pc' # Suc p2 # sfs) cd"
 
 theorem determinismf: "\<Sigma> \<leadsto>\<^sub>f \<Sigma>' \<Longrightarrow> \<Sigma> \<leadsto>\<^sub>f \<Sigma>'' \<Longrightarrow> \<Sigma>' = \<Sigma>''"
 proof (induction \<Sigma> \<Sigma>' rule: evalf.induct)
-  case (evf_lookup cd pc x env v h vs sfs)
+  case (evf_lookup cd pc x env p v h vs sfs)
   from evf_lookup(3, 1, 2) show ?case 
-    by (induction "FS h vs ((Suc pc # env) # sfs) cd" \<Sigma>'' rule: evalf.induct) simp_all 
+    by (induction "FS h env vs (Suc pc # p # sfs) cd" \<Sigma>'' rule: evalf.induct) simp_all 
 next
-  case (evf_pushcon cd pc k h h' v vs env sfs)
-  from evf_pushcon(3, 1, 2) show ?case 
-    by (induction "FS h vs ((Suc pc # env) # sfs) cd" \<Sigma>'' rule: evalf.induct) simp_all 
+  case (evf_pushcon cd pc k h h1 v h2 v' h3 v2 env vs p sfs)
+  from evf_pushcon(5, 1, 2, 3, 4) show ?case 
+    by (induction "FS h env vs (Suc pc # p # sfs) cd" \<Sigma>'' rule: evalf.induct) simp_all 
 next
-  case (evf_pushlam cd pc pc' h env h' v vs sfs)
-  from evf_pushlam(3, 1, 2) show ?case 
-    by (induction "FS h vs ((Suc pc # env) # sfs) cd" \<Sigma>'' rule: evalf.induct) simp_all 
+  case (evf_pushlam cd pc pc' h h1 v p h2 v' h3 v2 env vs sfs)
+  from evf_pushlam(5, 1, 2, 3, 4) show ?case 
+    by (induction "FS h env vs (Suc pc # p # sfs) cd" \<Sigma>'' rule: evalf.induct) simp_all 
 next
-  case (evf_apply cd pc h v2 env' pc' v1 vs env sfs)
-  from evf_apply(3, 1, 2) show ?case 
-    by (induction "FS h (v1 # v2 # vs) ((Suc pc # env) # sfs) cd" \<Sigma>'' rule: evalf.induct) 
-       simp_all 
+  case (evf_apply cd pc h v2 p' pc' env v1 env1 p1 env2 p2 vs p sfs)
+  from evf_apply(5, 1, 2, 3, 4) show ?case 
+    by (induction "FS h env (v1 # v2 # vs) (Suc pc # p # sfs) cd" \<Sigma>'' rule: evalf.induct) simp_all 
 next
-  case (evf_return cd pc h vs env sfs)
+  case (evf_return cd pc h env vs p sfs)
   from evf_return(2, 1) show ?case 
-    by (induction "FS h vs ((Suc pc # env) # sfs) cd" \<Sigma>'' rule: evalf.induct) simp_all 
+    by (induction "FS h env vs (Suc pc # p # sfs) cd" \<Sigma>'' rule: evalf.induct) simp_all 
 next
-  case (evf_jump cd pc h v2 env' pc' v1 vs env sfs)
-  from evf_jump(3, 1, 2) show ?case 
-    by (induction "FS h (v1 # v2 # vs) ((Suc pc # env) # sfs) cd" \<Sigma>'' rule: evalf.induct) 
-       simp_all 
+  case (evf_jump cd pc h v2 p' pc' env v1 env1 p1 env2 p2 vs p sfs)
+  from evf_jump(5, 1, 2, 3, 4) show ?case 
+    by (induction "FS h env (v1 # v2 # vs) (Suc pc # p # sfs) cd" \<Sigma>'' rule: evalf.induct) simp_all 
 qed
 
 lemma [simp]: "\<Sigma> \<leadsto>\<^sub>f \<Sigma>' \<Longrightarrow> code \<Sigma> = code \<Sigma>'"
