11FlatMemory/MemoryFlattening.thy
@@ -1,102 +1,21 @@
-theory MemoryFlattening
+theory MemoryFlattening                   
   imports FlatMemory "../09HeapMemory/HeapConversion"
 begin
 
-primrec splay_closure :: "(ptr \<Rightarrow> ptr) \<Rightarrow> hclosure \<Rightarrow> nat list" where
-  "splay_closure mp (HConst k) = [0, k]"
-| "splay_closure mp (HLam env pc) = Suc (length env) # pc # map mp env"
+primrec flatten :: "chained_state \<Rightarrow> flat_state" where
+  "flatten (CES h env vs sfs cd) = undefined"
 
-primrec flatten_closure :: "(ptr \<Rightarrow> ptr) \<Rightarrow> hclosure \<Rightarrow> hclosure" where
-  "flatten_closure mp (HConst k) = HConst k"
-| "flatten_closure mp (HLam env pc) = HLam (map mp env) pc"
-
-primrec flatten_frame :: "(ptr \<Rightarrow> ptr) \<Rightarrow> ptr list \<times> nat \<Rightarrow> nat list" where
-  "flatten_frame mp (env, pc) = pc # map mp env"
-
-primrec flatten :: "heap_state \<Rightarrow> flat_state" where
-  "flatten (HS h vs sfs cd) = (case hsplay splay_closure h of
-      (h', mp) \<Rightarrow> FS h' (map mp vs) (map (flatten_frame mp) sfs) cd)"
-
-theorem correctf: "flatten \<Sigma>\<^sub>h \<leadsto>\<^sub>f \<Sigma>\<^sub>f' \<Longrightarrow> \<exists>\<Sigma>\<^sub>h'. \<Sigma>\<^sub>h \<leadsto>\<^sub>h \<Sigma>\<^sub>h' \<and> flatten \<Sigma>\<^sub>h' = \<Sigma>\<^sub>f'" 
+theorem correctf: "flatten \<Sigma>\<^sub>c\<^sub>e \<leadsto>\<^sub>f \<Sigma>\<^sub>f' \<Longrightarrow> \<exists>\<Sigma>\<^sub>c\<^sub>e'. \<Sigma>\<^sub>c\<^sub>e \<leadsto>\<^sub>c\<^sub>e \<Sigma>\<^sub>c\<^sub>e' \<and> flatten \<Sigma>\<^sub>c\<^sub>e' = \<Sigma>\<^sub>f'" 
   by simp
 
-lemma [simp]: "stack_contains h vs \<Longrightarrow> hsplay splay_closure h = (h', mp) \<Longrightarrow> 
-  halloc h k = (h'', x) \<Longrightarrow> map (mp(x := y)) vs = map mp vs"
-proof (induction vs)
-  case (Cons v vs)
-  hence "x \<noteq> v" by simp
-  hence "v = x \<Longrightarrow> y = mp x" by simp
-  with Cons show ?case by simp
-qed simp_all
-
-lemma [simp]: "env_contains h envs \<Longrightarrow> hsplay splay_closure h = (h', mp) \<Longrightarrow>
-  halloc h k = (h'', x) \<Longrightarrow> 
-    map (map (mp(x := y))) envs = map (map mp) envs"
-  by (induction envs) (simp_all del: map_eq_conv, fastforce)
-
-lemma [simp]: "halloc_list h\<^sub>1 (splay_closure mp v) = (h\<^sub>2, y) \<Longrightarrow> 
-    get_closure h\<^sub>2 y = flatten_closure mp v"
-proof (induction v)
-  case (HConst x)
-  then obtain h' p' where "halloc h\<^sub>1 0 = (h', y) \<and> halloc h' x = (h\<^sub>2, p')" 
-    by (simp split: prod.splits)
-
-
-
-  hence "(case hlookup h\<^sub>2 y of 0 \<Rightarrow> HConst (hlookup h\<^sub>2 (Suc y))
-     | Suc x \<Rightarrow> HLam (hlookup_list h\<^sub>2 (Suc (Suc y)) x) (hlookup h\<^sub>2 (Suc y))) =
-    HConst x" by simp
-  then show ?case by simp
-next
-  case (HLam x1a x2)
-  then show ?case by simp
-qed
-
-lemma [simp]: "hsplay' splay_closure h hp = (h', mp) \<Longrightarrow> x < hp \<Longrightarrow> 
-    get_closure h' (mp x) = flatten_closure mp (h x)"
-proof (induction hp arbitrary: h' mp)
-  case (Suc hp)
-  then show ?case
-  proof (cases "x = hp")
-    case True
-    obtain h\<^sub>2 mp' where H: "hsplay' splay_closure h hp = (h\<^sub>2, mp')" by fastforce
-    obtain h\<^sub>3 y where Y: "halloc_list h\<^sub>2 (splay_closure mp' (h hp)) = (h\<^sub>3, y)" by fastforce 
-
-
-
-    with True have "get_closure h\<^sub>3 y = flatten_closure (mp'(hp := y)) (h x)" by simp
-    with True have "get_closure h\<^sub>3 ((mp'(hp := y)) x) = flatten_closure (mp'(hp := y)) (h x)"
-      by simp
-    with Suc H Y show ?thesis by simp
-  next
-    case False
-    obtain h\<^sub>2 mp' where H: "hsplay' splay_closure h hp = (h\<^sub>2, mp')" by fastforce
-    obtain h\<^sub>3 y where Y: "halloc_list h\<^sub>2 (splay_closure mp' (h hp)) = (h\<^sub>3, y)" by fastforce 
-  
-  
-    from Suc False H have "get_closure h\<^sub>2 (mp' x) = flatten_closure mp' (h x)" by simp
-    from Suc False have "x < hp" by simp
-  
-  
-    from False have "get_closure h\<^sub>3 ((mp'(hp := y)) x) = flatten_closure (mp'(hp := y)) (h x)" by simp
-    with Suc H Y show ?thesis by simp
-  qed
-qed simp_all
-
-lemma get_closure_flatten [simp]: "hsplay splay_closure h = (h', mp) \<Longrightarrow> hcontains h x \<Longrightarrow>
-    get_closure h' (mp x) = flatten_closure mp (hlookup h x)"
-  by (induction h) (simp_all del: get_closure.simps)
-
-theorem completef [simp]: "\<Sigma>\<^sub>h \<leadsto>\<^sub>h \<Sigma>\<^sub>h' \<Longrightarrow> heap_structured \<Sigma>\<^sub>h \<Longrightarrow> flatten \<Sigma>\<^sub>h \<leadsto>\<^sub>f flatten \<Sigma>\<^sub>h'" 
+theorem completef [simp]: "\<Sigma>\<^sub>c\<^sub>e \<leadsto>\<^sub>c\<^sub>e \<Sigma>\<^sub>c\<^sub>e' \<Longrightarrow> flatten \<Sigma>\<^sub>c\<^sub>e \<leadsto>\<^sub>f flatten \<Sigma>\<^sub>c\<^sub>e'" 
   by simp
 
-lemma completef_iter [simp]: "iter (\<leadsto>\<^sub>h) \<Sigma>\<^sub>h \<Sigma>\<^sub>h' \<Longrightarrow> heap_structured \<Sigma>\<^sub>h \<Longrightarrow>
-  iter (\<leadsto>\<^sub>f) (flatten \<Sigma>\<^sub>h) (flatten \<Sigma>\<^sub>h')"
-proof (induction \<Sigma>\<^sub>h \<Sigma>\<^sub>h' rule: iter.induct)
-  case (iter_step \<Sigma>\<^sub>h \<Sigma>\<^sub>h' \<Sigma>\<^sub>h'')
-  moreover hence "heap_structured \<Sigma>\<^sub>h'" by simp
-  ultimately have "iter (\<leadsto>\<^sub>f) (flatten \<Sigma>\<^sub>h') (flatten \<Sigma>\<^sub>h'')" by simp
-  moreover from iter_step have "flatten \<Sigma>\<^sub>h \<leadsto>\<^sub>f flatten \<Sigma>\<^sub>h'" by simp
+lemma completef_iter [simp]: "iter (\<leadsto>\<^sub>c\<^sub>e) \<Sigma>\<^sub>c\<^sub>e \<Sigma>\<^sub>c\<^sub>e' \<Longrightarrow> iter (\<leadsto>\<^sub>f) (flatten \<Sigma>\<^sub>c\<^sub>e) (flatten \<Sigma>\<^sub>c\<^sub>e')"
+proof (induction \<Sigma>\<^sub>c\<^sub>e \<Sigma>\<^sub>c\<^sub>e' rule: iter.induct)
+  case (iter_step \<Sigma>\<^sub>c\<^sub>e \<Sigma>\<^sub>c\<^sub>e' \<Sigma>\<^sub>c\<^sub>e'')
+  hence "iter (\<leadsto>\<^sub>f) (flatten \<Sigma>\<^sub>c\<^sub>e') (flatten \<Sigma>\<^sub>c\<^sub>e'')" by simp
+  moreover from iter_step have "flatten \<Sigma>\<^sub>c\<^sub>e \<leadsto>\<^sub>f flatten \<Sigma>\<^sub>c\<^sub>e'" by simp
   ultimately show ?case by simp
 qed simp_all
 
