09HeapMemory/Heap.thy
@@ -60,42 +60,6 @@ lemma halloc_map [simp]: "halloc h a = (h', v) \<Longrightarrow> halloc (hmap f 
 lemma [simp]: "hlookup (hmap f h) x = f (hlookup h x)"
   by (induction h) simp_all
 
-primrec halloc_list :: "'a heap \<Rightarrow> 'a list \<Rightarrow> 'a heap \<times> ptr" where
-  "halloc_list h [] = (h, undefined)"
-| "halloc_list h (x # xs) = (case halloc h x of
-      (h', p) \<Rightarrow> (case halloc_list h' xs of
-          (h'', p') \<Rightarrow> (h'', p)))"
-
-primrec hlookup_list :: "nat heap \<Rightarrow> ptr \<Rightarrow> nat \<Rightarrow> nat list" where
-  "hlookup_list h x 0 = []"
-| "hlookup_list h x (Suc n) = hlookup h x # hlookup_list h (Suc x) n"
-
-primrec hsplay' :: "((ptr \<Rightarrow> ptr) \<Rightarrow> 'a \<Rightarrow> 'b list) \<Rightarrow> (nat \<Rightarrow> 'a) \<Rightarrow> nat \<Rightarrow> 'b heap \<times> (ptr \<Rightarrow> ptr)" 
-    where
-  "hsplay' f h 0 = (hempty, \<lambda>x. undefined)"
-| "hsplay' f h (Suc hp) = (case hsplay' f h hp of
-      (h', mp) \<Rightarrow> (case halloc_list h' (f mp (h hp)) of
-          (h'', x) \<Rightarrow> (h'', mp(hp := x))))"
-
-fun hsplay :: "((ptr \<Rightarrow> ptr) \<Rightarrow> 'a \<Rightarrow> 'b list) \<Rightarrow> 'a heap \<Rightarrow> 'b heap \<times> (ptr \<Rightarrow> ptr)" where
-  "hsplay f (H h hp) = hsplay' f h hp"
-
-lemma [simp]: "halloc_list h vs = (h\<^sub>2, x) \<Longrightarrow> hcontains h y \<Longrightarrow> hlookup h\<^sub>2 y = hlookup h y"
-  by (induction vs arbitrary: h x) (auto split: prod.splits)
-
-lemma [simp]: "halloc_list h\<^sub>1 (v # vs) = (h\<^sub>2, x) \<Longrightarrow> hlookup h\<^sub>2 x = v"
-  by (induction h\<^sub>1) (simp split: prod.splits)
-
-lemma [simp]: "hsplay f hempty = (hempty, \<lambda>x. undefined)"
-  by (simp add: hempty_def)
-
-lemma [simp]: "x \<ge> hp \<Longrightarrow> hsplay' f (h(x := v)) hp = hsplay' f h hp"
-  by (induction hp) simp_all
-
-lemma [simp]: "halloc h v = (h', x) \<Longrightarrow> hsplay f h = (h\<^sub>1, mp) \<Longrightarrow> 
-    halloc_list h\<^sub>1 (f mp v) = (h\<^sub>2, y) \<Longrightarrow> hsplay f h' = (h\<^sub>2, mp(x := y))"
-  by (induction h) fastforce
-
 primrec stack_contains :: "'a heap \<Rightarrow> ptr list \<Rightarrow> bool" where
   "stack_contains h [] = True"
 | "stack_contains h (v # vs) = (hcontains h v \<and> stack_contains h vs)"
