10ChainedEnvironment/Chaining.thy
@@ -1,0 +1,53 @@
+theory Chaining
+  imports ChainedEnvironment "../09HeapMemory/HeapMemory"
+begin
+
+definition unstack_list :: "(ptr \<times> ptr) heap \<Rightarrow> ptr \<Rightarrow> ptr list" where
+  "unstack_list env p = undefined"
+
+definition unchain_heap :: "ceclosure heap \<Rightarrow> (ptr \<times> ptr) heap \<Rightarrow> hclosure heap" where
+  "unchain_heap h env = undefined"
+
+primrec unchain_frame :: "(ptr \<times> ptr) heap \<Rightarrow> (ptr \<times> nat) \<Rightarrow> (ptr list \<times> nat)" where
+  "unchain_frame env (p, pc) = (unstack_list env p, pc)"
+
+abbreviation unchain_stack :: "(ptr \<times> ptr) heap \<Rightarrow> (ptr \<times> nat) list \<Rightarrow> (ptr list \<times> nat) list" where
+  "unchain_stack env sfs \<equiv> map (unchain_frame env) sfs"
+
+primrec unchain_state :: "chained_state \<Rightarrow> heap_state" where
+  "unchain_state (CES h env vs sfs cd) = HS (unchain_heap h env) vs (unchain_stack env sfs) cd"
+
+lemma [simp]: "lookup (unstack_list env p) x = chain_lookup env p x"
+  by simp
+
+lemma [simp]: "halloc h (CEConst k) = (h', p) \<Longrightarrow> 
+    halloc (unchain_heap h env) (HConst k) = (unchain_heap h' env, p)"
+  by simp
+
+lemma [simp]: "halloc h (CELam p pc) = (h', v) \<Longrightarrow> 
+    halloc (unchain_heap h env) (HLam (unstack_list env p) pc) = (unchain_heap h' env, v)"
+  by simp
+
+theorem completece [simp]: "unchain_state \<Sigma>\<^sub>c\<^sub>e \<leadsto>\<^sub>h \<Sigma>\<^sub>h \<Longrightarrow> \<exists>\<Sigma>\<^sub>c\<^sub>e'. \<Sigma>\<^sub>c\<^sub>e \<leadsto>\<^sub>c\<^sub>e \<Sigma>\<^sub>c\<^sub>e' \<and> \<Sigma>\<^sub>h = unchain_state \<Sigma>\<^sub>c\<^sub>e'"
+  by simp
+
+theorem correctce [simp]: "\<Sigma>\<^sub>c\<^sub>e \<leadsto>\<^sub>c\<^sub>e \<Sigma>\<^sub>c\<^sub>e' \<Longrightarrow> unchain_state \<Sigma>\<^sub>c\<^sub>e \<leadsto>\<^sub>h unchain_state \<Sigma>\<^sub>c\<^sub>e'"
+proof (induction \<Sigma>\<^sub>c\<^sub>e \<Sigma>\<^sub>c\<^sub>e' rule: evalce.induct)
+  case (evce_apply cd pc h v2 p' pc' env v1 env' p'' vs p sfs)
+  from evce_apply have "cd ! pc = BApply" by simp
+  from evce_apply have "hlookup h v2 = CELam p' pc'" by simp
+  from evce_apply have "halloc env (v1, p') = (env', p'')" by simp
+
+  from evce_apply have "hlookup (unchain_heap h env) v2 = HLam (unstack_list env p') pc' \<Longrightarrow>
+        HS (unchain_heap h env) (v1 # v2 # vs) ((unstack_list env p, Suc pc) # unchain_stack env sfs) cd \<leadsto>\<^sub>h
+    HS (unchain_heap h env) vs ((v1 # unstack_list env p', pc') # (unstack_list env p, pc) # unchain_stack env sfs) cd" by simp
+
+  have "HS (unchain_heap h env) (v1 # v2 # vs) ((unstack_list env p, Suc pc) # unchain_stack env sfs) cd \<leadsto>\<^sub>h
+    HS (unchain_heap h env') vs ((unstack_list env' p'', pc') # (unstack_list env' p, pc) # unchain_stack env' sfs) cd" by simp
+  then show ?case by simp
+next
+  case (evce_jump cd pc h v2 p' pc' env v1 env' p'' vs p sfs)
+  then show ?case by simp
+qed simp_all
+
+end
